\documentclass[12pt,letterpaper]{article}

\usepackage{amsmath}
\usepackage{amssymb}
\usepackage{amsthm}
\usepackage{commath}
\usepackage{hyperref}

\begin{document}
	\section*{Input}
		\[\int 4x^2 \dif x\]
	\section*{Output}
		\subsection*{Step 1}
			We start by using the \nameref{sec:constmulrule}:
			\[\int af(x) \dif x = a \int f(x) \dif x\]
			So:
			\[\int 4x^2 \dif x = 4 \int x^2 \dif x\]
		\subsection*{Step 2}
			Next, we find $\int x^2 \dif x$ using the \nameref{sec:powerrule}:
			\[\int x^a \dif x = \frac{x^{a+1}}{a+1}\]
			\[\int x^2 \dif x = \frac{x^3}{3}\]
		\subsection*{Final step}
			\[\int 4x^2 \dif x = 4 \int x^2 \dif x = \frac{4x^3}{3}\]
	\newpage
	\appendix
	\section{Constant multiple rule}\label{sec:constmulrule}
		We can prove that $\int af(x) \dif x = a \int f(x) \dif x$.
		\begin{proof}
			Let $F(x) = \int f(x) \dif x$.

			We know that:
			\[\left(aF(x)\right)' = a F'(x) = a f(x)\]
			From here we can prove the constant multiple rule:
			\begin{align*}
				\left(a F(x)\right)' &= a f(x)\\
				a F(x) &= \int a f(x) \dif x\\
				a \int f(x) \dif x &= \int a f(x) \dif x
			\end{align*}
		\end{proof}
	\section{Power rule}\label{sec:powerrule}
		We can prove that $\int x^a \dif x = \frac{x^{a+1}}{a+1}$.
		\begin{proof}
			We will do this by finding $\left(\frac{x^{a+1}}{a+1}\right)$:
			\[\left(\frac{x^{a+1}}{a+1}\right)' = \frac{(a+1)(a+1)(x^a)}{(a+1)^2} = x^a\]
		\end{proof}
\end{document}
